comparing Mikes and my statements of the axioms; deriving the second computation rule as a lemma

Experimental/Pi0.v
@@ -9,6 +9,14 @@ Require Import Menagerie.
 Definition isProp (X:Type) := forall {x y : X}, x ~~> y.
 Definition isSet (X:Type) := forall {x y : X}, isProp (x ~~> y). 
 
+Lemma prop_implies_set : forall {X:Type}, isProp X -> isSet X.
+Admitted.
+
+Lemma set_implies_hlevel_3 : forall {X:Type}, isSet X -> forall {x y : X}, isSet (x ~~> y).
+Proof.
+  intros X XisSet x y.  apply prop_implies_set.  apply XisSet.
+Defined.
+
 Lemma transp_along_map_on_paths : forall {Y X : Type} {P : X -> Type}
                                          {f : Y -> X}
                                          {y y':Y} {u:y~~>y'}
@@ -44,30 +52,30 @@ Admitted.
 
 (*
 Inductive pi0 (X:Type) : Type :=
-    | cmpt : X -> pi0 X
-    | contr : forall (l : Circle -> pi0 X), paths (idpath (l base)) (cong l loop)
+    | pi0_cmpt : X -> pi0 X
+    | pi0_contr : forall (l : Circle -> pi0 X), paths (idpath (l base)) (cong l loop)
 *)
 
 Axiom pi0 : Type -> Type.
 
-Axiom cmpt : forall {X} (x:X), (pi0 X).
+Axiom pi0_cmpt : forall {X} (x:X), (pi0 X).
 
-Axiom contr : forall {X} (l : Circle -> (pi0 X)), (map_on_paths l loop) ~~> (idpath (l base)).
+Axiom pi0_contr : forall {X} (l : Circle -> (pi0 X)), (map_on_paths l loop) ~~> (idpath (l base)).
 
 
 
 Axiom pi0_rect : forall {X} {P : (pi0 X -> Type)}
-                    (d_cmpt : forall x:X, P (cmpt x))
+                    (d_cmpt : forall x:X, P (pi0_cmpt x))
                     (d_contr : forall (l : Circle -> (pi0 X))  (k : forall a:Circle, P (l a)),
                       let id_coerced_along_contr :=
                          ( transp_along_map_on_paths
-                         @ (map_on_paths (fun u : l base ~~> l base => transport u (k base)) (contr l)) )
+                         @ (map_on_paths (fun u : l base ~~> l base => transport u (k base)) (pi0_contr l)) )
                       in
                          (id_coerced_along_contr) ~~> (dependent_map_on_paths k loop)),
                  forall (z : pi0 X), P z.
 
 Axiom pi0_comp_cmpt : forall {X} {P} {d_cmpt} {d_contr} (x:X),
-                             (@pi0_rect X P d_cmpt d_contr (cmpt x)) ~~> (d_cmpt x). 
+                             (@pi0_rect X P d_cmpt d_contr (pi0_cmpt x)) ~~> (d_cmpt x). 
 
 (* Axiom pi0_comp_contr *)
 (* Horrible to type… but actually should be redundant for homotopical reasons anyway, I think, so hopefully leaving it out will not hurt us. *)
@@ -78,11 +86,12 @@ Proof.
   apply (@pi0_rect X (fun _ => Y) f); intros.  apply s.
 Defined.
 
-Lemma pi0_nondep_comp : forall {X} {Y} {s} {f} (x:X), (@pi0_nondep_rect X Y s f (cmpt x) ~~> (f x)).
+Lemma pi0_nondep_comp_base : forall {X} {Y} {s} {f} (x:X), (@pi0_nondep_rect X Y s f (pi0_cmpt x) ~~> (f x)).
 Proof.
   intros; unfold pi0_nondep_rect.  exact (pi0_comp_cmpt (P := fun _ => Y) x).
 Defined.  (* maybe could/should leave opaque, since is a path in a set? *)
 
+(* Again, pi0_nondep_comp_loop is unnecessary, since we can get its result equivalently and more directly from the fact that Y is a set. *)
 
 Lemma if_circles_contract_then_loops_contract {X : Type} :
         (forall (l : Circle -> X), (map_on_paths l loop) ~~> (idpath (l base)))
@@ -110,7 +119,7 @@ Proof.
     (* units/inverses dealt with automagically in both subgoals *)
 Defined.
 
-Lemma if_loops_contract_then_isset {X : Type} :
+Lemma if_loops_contract_then_is_set {X : Type} :
         (forall (x:X) (p : x ~~> x), (p ~~> idpath x)) 
         -> isSet X.
 Proof.
@@ -125,3 +134,128 @@ solved in the following 3 lines respectively: *)
   apply opposite; apply concat_associativity.
   path_via (idpath _ @ v).  (* both subgoals auto (by: contr ; unitarity) *)
 Defined.
+
+Lemma if_is_set_then_circles_contract : forall {X : Type}, isSet X -> 
+           (forall (l : Circle -> X), (map_on_paths l loop) ~~> (idpath (l base))).
+Proof.
+  intros X isSetX l.  apply isSetX.
+Defined.
+
+Lemma pi0_is_set : forall {X:Type}, isSet (pi0 X).
+Proof.
+  intros X.
+  apply if_loops_contract_then_is_set.
+  apply if_circles_contract_then_loops_contract.
+  exact pi0_contr.
+Defined.
+
+
+
+
+
+(* Deriving Mike’s statements of the axioms from mine: *)
+
+Definition map_dep {A} {P} f {x y} p := @dependent_map_on_paths A P f x y p.
+
+(* Definition pi0 {X:Type} — already defined. *)
+
+Definition pi0_cpnt {X} := @pi0_cmpt X.
+
+Lemma pi0_axiomK : forall {A : Type} (x : pi0 A) (l : x ~~> x), l ~~> idpath x.
+Proof.
+  intros A.  apply if_circles_contract_then_loops_contract.  exact pi0_contr.
+Defined.    
+
+(* what Mike’s calling “axiom K” is what I’ve been calling “loops contract” *)
+
+Lemma fibred_K_implies_loops_contract_in_fibres :
+  forall {X : Type} {axiomK : forall (x : X) (l : x ~~> x), l ~~> idpath x}
+         {P : X -> Type}
+         (fibred_K : forall (x : X) (l : x ~~> x) (z : P x)
+                            (dl : transport l z ~~> z),
+                    dl ~~> map (fun p: x ~~> x => transport p z) (axiomK x l)),
+  forall (x : X) (z : P x) (p : z ~~> z), p ~~> idpath z.
+Proof.
+  intros X axiomK P fibred_K x z p.
+  exact ((fibred_K x (idpath x) z p) @ ! (fibred_K x (idpath x) z (idpath z))). 
+Defined.
+
+Lemma pi0_rect' :
+  forall {A : Type} {P : pi0 A -> Type}
+         (dcpnt : forall (x : A), P (pi0_cpnt x))
+         (daxiomK : forall (x : pi0 A) (l : x ~~> x) (z : P x)
+                           (dl : transport l z ~~> z),
+                    dl ~~> map (fun p: x ~~> x => transport p z) (pi0_axiomK x l)),
+  forall (x : pi0 A), P x.
+Proof.
+  intros A P dcpnt daxiomK.  apply (@pi0_rect A P dcpnt).
+(* The only non-trivial hypothesis for pi0_rect is ‘d_contr’. *)
+(* For this, we need a lemma: *)
+  assert (forall (x : pi0 A), isSet (P x)) as fibres_are_sets.
+    intros x.
+    apply if_loops_contract_then_is_set.
+    apply (fibred_K_implies_loops_contract_in_fibres (axiomK := pi0_axiomK)).  
+    assumption.
+(* Now we can easily construct ‘d_contr’:*)
+  intros l k; apply fibres_are_sets.
+Defined.
+
+Lemma pi0'_compute_cpnt :
+  forall {A : Type} {P : pi0 A -> Type}
+         (dcpnt : forall (x : A), P (pi0_cpnt x))
+         (daxiomK : forall (x : pi0 A) (l : x ~~> x) (z : P x)
+                           (dl : transport l z ~~> z),
+                    dl ~~> map (fun p: x ~~> x => transport p z) (pi0_axiomK x l))
+         (a : A),
+  pi0_rect' dcpnt daxiomK (pi0_cpnt a) ~~> dcpnt a.
+Proof.
+  intros A P dpnt daxiomK a.
+  apply pi0_comp_cmpt.
+Defined.
+ 
+Definition map2_dep {X : Type} {P : X -> Type} {x y : X} {p q : x ~~> y}
+ (f : forall x, P x) (s : p ~~> q) :
+ map_dep f p ~~> map (fun p : x ~~> y => transport p (f x)) s @ map_dep f q.
+Proof.
+ path_induction.
+Defined.
+
+Definition map2_dep_loop {X : Type} {P : X -> Type} {x : X} {l : x ~~> x}
+ (f : forall x, P x) (s : l ~~> idpath x) :
+ map_dep f l ~~> map (fun p : x ~~> x => transport p (f x)) s.
+Proof.
+(* intros X P x l f s. *)
+ match goal with |- _ ~~> ?t => path_via (t @ map_dep f (idpath x)) end.
+ apply map2_dep.
+(* not needed by Mike: *)
+ simpl.  path_tricks.
+Defined.
+
+Lemma pi0_compute_axiomK : 
+  forall {A : Type} {P : pi0 A -> Type}
+         (dcpnt : forall (x : A), P (pi0_cpnt x))
+         (daxiomK : forall (x : pi0 A) (l : x ~~> x) (z : P x)
+                           (dl : transport l z ~~> z),
+                    dl ~~> map (fun p: x ~~> x => transport p z) (pi0_axiomK x l))
+         (x : pi0 A) (l : x ~~> x),
+    map2_dep_loop (pi0_rect' dcpnt daxiomK) (pi0_axiomK x l)
+  ~~>
+    daxiomK x l (pi0_rect' dcpnt daxiomK x) (map_dep (pi0_rect' dcpnt daxiomK) l).
+Proof.
+  intros A P dcpnt daxiomk.
+  assert (forall (x : pi0 A), isSet (P x)) as fibres_are_sets.
+    intros x.
+    apply if_loops_contract_then_is_set.
+    apply (fibred_K_implies_loops_contract_in_fibres (axiomK := pi0_axiomK)).
+    assumption.
+  assert (forall (x : pi0 A) (z z' : P x), isSet (z ~~> z')) as fibres_are_hlevel_3.
+    intros x.
+    apply set_implies_hlevel_3.
+    apply fibres_are_sets.
+  intros x l.  apply fibres_are_hlevel_3.
+Defined.
+(* This proof can be shortened a bit, β-reducing the first assertion within the second; but I think this separation is a little more perspicuous. *)
+
+
+
+
